Formal Methods/dafny/hoare/ex2.dfy
@@ -1,0 +1,16 @@
+method Main()
+{
+    var x:int, y:int;
+
+    assume x > 2 && y > 3;
+
+    assert y + x + 1 > 6;
+    
+    x := x+1;
+
+    assert y+x > 6;
+
+    y := y+x;
+
+    assert y > 6;
+}
