Formal Methods/dafny/hoare/ex3.dfy
@@ -1,0 +1,10 @@
+method Main()
+{
+    var x:int;
+
+    if x < 0
+    {
+        x := -x;
+    }
+    assert x >= 0;
+}
