Formal Methods/dafny/hoare/ex4.dfy
@@ -1,0 +1,9 @@
+method Main()
+{
+    var i:int;
+    while i>0
+    {
+        i := i - 1;
+    }
+    assert i <= 0;
+}
